finished create_IOLTS and create_s_IOLTS

src/IOTS.v
@@ -3,49 +3,104 @@ Require Import Coq.Lists.List.
 Require Import Coq.Lists.ListSet.
 Import Coq.Lists.List.ListNotations.
 Require Import RelationClasses.
+Require Import BE_ltacs.
+Require Import String.
+Require Import Bool.
 
 Open Scope list_scope.
 
 (* Definição 6*)
 Section SectionIOLTS.
 
-  Fixpoint is_disjoint (l m : list label) : Prop :=
-    match l with
-    | []      =>  True
-    | h :: t  =>  ~ In h m /\ is_disjoint t m
-    end.
+  Definition is_disjoint (L_i L_u : list label) : Prop :=
+    Forall (fun x => ~ In x L_u) L_i.
 
   Record IOLTS : Type := mkIOLTS {
       lts : LTS
     ; L_i : list label
     ; L_u : list label
     ; disjoint_input_output_labels  : is_disjoint L_i L_u
-    ; is_IOLTS                       : is_valid_LTS (L_i ++ L_u) lts
+    ; is_IOLTS                      : (L_i ++ L_u) = lts.(L)
     ; no_repetition_L_i             : NoDup L_i
     ; no_repetition_L_u             : NoDup L_u
   }.
-  
-  Definition create_IOLTS (lts : LTS) (Li Lu : list label) : option IOLTS. Admitted.
-  
+
+  Lemma is_disjoint_dec :
+    forall (Li Lu : set label), {is_disjoint Li Lu} + {~ is_disjoint Li Lu}.
+  Proof.
+    intros Li Lu. unfold is_disjoint. apply Forall_dec.
+    intros x. pose proof (in_dec string_dec x Lu) as in_dec. inversion in_dec.
+    - right. unfold not. intros H'. auto.
+    - left. auto.
+  Qed.
+
+  Lemma NoDup_dec :
+    forall {A : Type} (l : list A),
+    (forall a1 a2 : A, { a1 = a2 } + { a1 <> a2 }) ->
+     { NoDup l } + { ~ NoDup l }.
+  Proof.
+    intros A l Aeq_dec. induction l as [| h l' H].
+    - left. apply NoDup_nil.
+    - inversion H.
+      + pose proof (in_dec Aeq_dec h l') as H'. inversion H'.
+        * right. intros H''. inversion H''. auto.
+        * left. apply NoDup_cons; auto.
+      + right. intros H'. inversion H'. auto.
+  Qed.
+
+  Definition create_IOLTS (lts : LTS) (Li Lu : list label) : option IOLTS :=
+    match is_disjoint_dec Li Lu with
+    | left h_is_disjoint =>
+        match list_eq_dec string_dec (Li ++ Lu) lts.(L) with
+        | left h_is_IOLTS =>
+            match NoDup_dec Li string_dec with
+            | left h_NoDup_Li =>
+                match NoDup_dec Lu string_dec with
+                | left h_NoDup_Lu =>
+                    Some (mkIOLTS
+                            lts
+                            Li
+                            Lu
+                            h_is_disjoint
+                            h_is_IOLTS
+                            h_NoDup_Li
+                            h_NoDup_Lu)
+                | right _ => None
+                end
+            | right _ => None
+            end
+        | right _ => None
+        end
+    | right _ => None
+    end.
+
   Theorem create_IOLTS_correct :
     forall (lts : LTS) (L_i L_u : list label),
-      is_disjoint L_i L_u /\ is_valid_LTS (L_i ++ L_u) lts /\ NoDup L_i /\ NoDup L_u
+      is_disjoint L_i L_u /\ (L_i ++ L_u) = lts.(L) /\ NoDup L_i /\ NoDup L_u
       -> create_IOLTS lts L_i L_u <> None.
-  Proof. Admitted.
-  
+  Proof.
+    intros lts Li Lu H. destruct H as [H [H2 [H3 H4]]].
+    unfold create_IOLTS. destruct (is_disjoint_dec Li Lu);auto.
+    destruct (list_eq_dec string_dec (Li ++ Lu) lts.(L));auto.
+    destruct (NoDup_dec Li string_dec);auto.
+    destruct (NoDup_dec Lu string_dec);auto.
+    unfold not. intros H5. inversion H5.
+  Qed.
 End SectionIOLTS.
 
 (* Definição 7*)
 Section SectionIOTS.
 
-  Fixpoint elem_reaches_another_with_all_labels (s : state) (ll : set label) (p : LTS) : Prop :=
+  Fixpoint elem_reaches_another_with_all_labels (s : state) (ll : set label)
+    (p : LTS) : Prop :=
   match ll with
   | []      =>  True
   | l :: t  =>  ind_has_reachability_to_some_other s [l] p /\
                          elem_reaches_another_with_all_labels s t p
   end.
 
-  Fixpoint every_elem_reaches_some_other (ls : set state) (ll : set label) (p : LTS) : Prop :=
+  Fixpoint every_elem_reaches_some_other (ls : set state) (ll : set label)
+    (p : LTS) : Prop :=
   match ls with
   | []      =>  True
   | h :: t  =>  elem_reaches_another_with_all_labels h ll p /\
@@ -74,20 +129,18 @@ Ltac empty_reachability_left := left; reflexivity.
 (* Definição 8*)
 Inductive ind_quiescent : state -> IOLTS -> Prop :=
 | quiescent_r1 : forall (s : state) (p : IOLTS),
-                      (forall (s' : state) (l : label),
-                          In l p.(L_u) /\ In s' p.(lts).(Q) ->
-                          ~ ind_transition s (event l) s' p.(lts)) -> ind_quiescent s p
-| quiescent_r2 : forall (s : state) (p : IOLTS),
-                      (forall (s' : state),
-                          In s' p.(lts).(Q) ->
-                          ~ ind_transition s tau s' p.(lts)) -> ind_quiescent s p.
+              (forall (s' : state) (l : label),
+                  In l p.(L_u) ->
+                  ~ ind_transition s (event l) s' p.(lts))->
+                  (forall (s' : state),
+                  ~ ind_transition s tau s' p.(lts)) -> ind_quiescent s p.
 
 Inductive ind_quiescent_traces : list label -> IOLTS -> Prop :=
 | quiescent_trace_r1  : forall (ll : list label) (p : IOLTS) (ls : set state),
-                                ind_traces_LTS ll p.(lts) /\
-                                    ind_after_LTS ll ls p.(lts) /\
-                                        (exists (s : state), In s ls /\ 
-                                            ind_quiescent s p) ->  ind_quiescent_traces ll p.
+                ind_traces_LTS ll p.(lts) /\
+                    ind_after_LTS ll ls p.(lts) /\
+                        (exists (s : state), In s ls /\ 
+                            ind_quiescent s p) ->  ind_quiescent_traces ll p.
 
 (* Definição 9*)
 Section SectionSuspensionIOLTS.
@@ -99,58 +152,109 @@ Section SectionSuspensionIOLTS.
 
   Record s_IOLTS : Type := mksIOLTS {
       iolts               : IOLTS
-    ; Ts                  :  list (state * delta_label * state)
+    ; Ts                  :  list (state)
     (*; Q_del                 :=  iolts.(lts).(Q)*)
     (*; L_del                 :=  set_union string_dec s_iolts.(lts).(L) [delta]*)
     (*; Li_del                :=  s_iolts.(L_i)*)
     (*; Lu_del                :=  set_union string_dec s_iolts.(L_u) [delta]*)
     (*; T_del                 :=  s_iolts.(lts).(T) ++ Ts*)
     (*; delta_not_in_L        : ~ In delta s_iolts.(lts).(L)*)
-    ; valid_del_transitions : forall (s s' : state) (l : delta_label), 
-                                        In (s, l, s') Ts -> s = s' /\ l = delta /\ In s iolts.(lts).(Q)
-    ; Ts_complete_correct   : forall (s : state), In (s, delta, s) Ts <-> In s iolts.(lts).(Q) /\
+    ; valid_del_transitions : forall (s : state), 
+                                        In s Ts -> In s iolts.(lts).(Q)
+    ; Ts_complete_correct   : forall (s : state), In s Ts <-> In s iolts.(lts).(Q) /\
                                         ind_quiescent s iolts
   }.
-  
-  Definition create_s_IOLTS (iolts : IOLTS) : s_IOLTS. Admitted.
-  
+
+  Definition out_transition (q : state) (Lu : set label)
+      (t : state * transition_label * state) : bool :=
+    match t with
+    | (q1, e, q2) =>
+        if Nat.eqb q1 q
+        then
+          match e with
+          | tau => true
+          | event e' => set_mem string_dec e' Lu
+          end
+        else false
+    end.
+
+  Definition is_quiescent (l : list (state * transition_label * state))
+      (Lu : list label) (q : state) : bool :=
+    negb (existsb (out_transition q Lu) l).
+
+  Definition create_Ts (iolts : IOLTS) : list state :=
+    filter (is_quiescent iolts.(lts).(T) iolts.(L_u)) iolts.(lts).(Q).
+
+  Lemma create_Ts_valid_del_transitions :
+    forall (iolts : IOLTS) (s : state), In s (create_Ts iolts) -> In s iolts.(lts).(Q).
+  Proof.
+    intros iolts s H. unfold create_Ts in H. apply filter_In in H.
+    destruct H as [H _]. apply H.
+  Qed.
+
+  Lemma existsb_false:
+    forall (A : Type) (f : A -> bool) (l : list A),
+      existsb f l = false <-> ~ exists x : A, In x l /\ f x = true.
+  Proof.
+    intros. split.
+    - intros H. pose proof (existsb_exists f l) as H'. apply iff_sym in H'.
+      apply Bool.iff_reflect in H'. rewrite H in H'. inversion H'. auto.
+    - intros H. pose proof (existsb_exists f l) as H'. apply iff_sym in H'.
+      apply Bool.iff_reflect in H'. inversion H'.
+      + unfold not in H. destruct H. apply H1.
+      + reflexivity.
+  Qed.
+
+  Lemma create_Ts_complete_correct :
+    forall (iolts : IOLTS) (s : state), 
+      In s (create_Ts iolts) <-> In s iolts.(lts).(Q) /\ ind_quiescent s iolts.
+  Proof.
+    intros iolts s. split.
+    - intros H. split.
+      + apply create_Ts_valid_del_transitions. apply H.
+      + apply filter_In in H. destruct H as [_ H].
+        apply quiescent_r1; [intros s' l H' | intros s'];
+        apply negb_true_iff in H; apply existsb_false in H; unfold not;
+        intros H''; apply H; inversion H'';
+        [ exists (s, event l, s') | exists (s, tau, s')];
+        split; auto; simpl; rewrite PeanoNat.Nat.eqb_refl;
+        [ apply (set_mem_correct2 string_dec); apply H' |
+          reflexivity ].
+    - intros H. destruct H as [H H']. apply filter_In. split.
+      + apply H.
+      + apply negb_true_iff. apply existsb_false. unfold not.
+        intros H''. destruct H'' as [x H'']. destruct H'' as [H'' H'''].
+        destruct x as [[q0 e] q1]. simpl in H'''.
+        destruct (Nat.eqb q0 s) eqn: EQ.
+        * apply EqNat.beq_nat_true in EQ. rewrite EQ in H''. inversion H'.
+          destruct e.
+          -- apply set_mem_correct1 in H'''. specialize (H0 q1 l).
+             destruct H0; auto. apply transition_r1; auto.
+          -- clear H'''. specialize (H1 q1). destruct H1.
+             apply transition_r2. auto.
+        * inversion H'''.
+  Qed.
+
+  Definition create_s_IOLTS (iolts : IOLTS) : s_IOLTS :=
+    mksIOLTS
+      iolts
+      (create_Ts iolts)
+      (create_Ts_valid_del_transitions iolts)
+      (create_Ts_complete_correct iolts).
+
   Theorem create_s_IOLTS_correct :
     forall (iolts : IOLTS), exists (s_iolts : s_IOLTS),
       create_s_IOLTS iolts = s_iolts.
-  Proof. Admitted.
-    
-End SectionSuspensionIOLTS.
+  Proof.
+    intros iolts. exists (create_s_IOLTS iolts). reflexivity.
+  Qed.
 
-Ltac all_delta_trans := intros s s' l A;
-    repeat(inversion A as [B|B];
-             [inversion B; split; [reflexivity | split; [reflexivity | t_elem_in_list]] | ];
-           clear A; rename B into A); inversion A.
-           
-Ltac all_quiescent_trans_incl := intros B;
-    repeat(inversion B as [C|C];
-      [inversion C ;
-        split;
-        [t_elem_in_list
-        |apply quiescent_r1; intros s' l D; destruct D as [D E];
-         repeat(inversion D as [F|F];
-           [repeat(inversion E as [G|G];
-             [subst l;
-              subst s';
-              unfold not;
-              intro H';
-              inversion H' as [I J K L M];
-              destruct M as [N [O [P Q]]];
-              repeat(inversion Q as [R|R];
-               [inversion R |]; clear Q; rename R into Q); inversion Q
-             |]; clear E; rename G into E); inversion E
-           |]; clear D; rename F into D); inversion D
-        ]
-      |]; clear B; rename C into B); inversion B.
+End SectionSuspensionIOLTS.
 
 Inductive ind_s_traces : state -> list label -> s_IOLTS -> Prop :=
 | s_traces_r1 : forall (s : state) (t : list label) (p : s_IOLTS),
-                   ind_traces s t p.(s_iolts).(lts) -> ind_s_traces s t p.
+                   ind_traces s t p.(iolts).(lts) -> ind_s_traces s t p.
 
 Inductive ind_s_traces_LTS : list label -> s_IOLTS -> Prop :=
 | s_traces_LTS_r1 : forall (t : list label) (p : s_IOLTS),
-                   ind_traces_LTS t p.(s_iolts).(lts) -> ind_s_traces_LTS t p.
+                   ind_traces_LTS t p.(iolts).(lts) -> ind_s_traces_LTS t p.
